Calculator.lean
@@ -1,1 +1,2 @@
-import Calculator.Basic
+import Calculator.Example
+import Calculator.ExampleRel
