Calculator/Implication.lean
@@ -1,0 +1,19 @@
+import Mathlib.Tactic.Common
+
+namespace Calculator.Syntax.Implication
+
+def impR (a b : Prop) : Prop := b -> a
+
+infix:25 "
+  <-
+" => impR
+
+@[simp, refl] theorem rfl_impR (a) : a <- a := by
+  unfold impR
+  exact id
+
+instance : IsTrans Prop impR where trans _ _ _ p q := p ∘ q
+instance : Std.Refl impR where refl := rfl_impR
+instance : IsPreorder Prop impR where
+
+namespace Calculator.Syntax.Implication
